Hybrid_Programs/Verification_Examples/RoboSim.thy
@@ -6,6 +6,7 @@ begin
 
 expr_vars
 
+(*
 method hoare_help =
   (
     (
@@ -21,7 +22,9 @@ method hoare_help =
        )
      )+, 
    (subst WHILE_unroll_IF[symmetric])?
-  )+
+  )+*)
+
+section \<open> RoboSim \<close>
 
 text \<open> Modelling components that are common to all RoboSim models. \<close>
 
@@ -38,8 +41,15 @@ dataspace robosim =
 context robosim
 begin
 
-abbreviation "T(P) \<equiv> IF \<not> wait THEN P ELSE skip"
-                                       
+subsection \<open> Time modelling \<close>
+
+text \<open> Every ODE will contain both a timer and a t variable for specification purposes,
+       so below we define TimerEvo that includes the lenses for t and timer, and moreover
+       specifies that these evolve at rate 1. The overall ODE system is then evolved within
+       timer \<le> \<delta> time, assuming timer has been set to 0 initially.  \<close>
+
+subsubsection \<open> TimerEvo \<close>
+
 definition "TimerEvo \<delta> a \<sigma> B \<equiv> g_dl_ode_frame (t +\<^sub>L timer +\<^sub>L a) (\<sigma>(t  \<leadsto> 1, timer \<leadsto> 1)) (@B \<and> $timer \<le> \<guillemotleft>\<delta>\<guillemotright>)\<^sub>e"
 
 lemma TimerEvo_delta_nmods:
@@ -53,38 +63,53 @@ lemma TimerEvo_pos_timer_delta:
   shows "\<^bold>{ P \<^bold>} TimerEvo \<delta> a \<sigma> B \<^bold>{ $timer \<le> \<guillemotleft>\<delta>\<guillemotright> \<^bold>}"
   using TimerEvo_def
   by (smt (verit, best) SEXP_def fbox_g_orbital_on predicate1I)
- 
+
+subsubsection \<open> EvolveUntil \<close>
+
+text \<open> Having defined the above, we are now in a position to specify a program that evolves
+       exactly until \<delta>. To ensure that sequential composition has the correct meaning, we 
+       introduce the function T(_) that behaves like healthiness condition R3 of the
+       theory of reactive processes. \<close>
+
+definition "T(P) \<equiv> IF \<not> wait THEN P ELSE skip"
+
+lemma hoare_T_wait:
+  assumes "\<^bold>{P \<and> \<not> wait\<^bold>} C \<^bold>{Q\<^bold>}" "`(P \<and> wait) \<longrightarrow> Q`"
+  shows "\<^bold>{P\<^bold>} T C \<^bold>{Q\<^bold>}"
+  unfolding T_def apply (rule hoare_if_then_else)
+  using assms apply simp
+  by (metis (mono_tags, lifting) SEXP_def assms(2) fbox_skip predicate1I taut_def)
+
+lemma hoare_T_wait':
+  assumes "\<^bold>{P\<^bold>} C \<^bold>{Q\<^bold>}"
+  shows "\<^bold>{P \<and> \<not> wait\<^bold>} T C \<^bold>{Q\<^bold>}"
+  unfolding T_def
+  using assms by fastforce
+
+lemma T_idempotent:"T(T(P)) = T(P)"
+  unfolding T_def
+  unfolding ifthenelse_def apply auto
+  by wlp_full
+
+text \<open> EvolveUntil is then defined using wait as follows. Initially timer is set to 0, wait
+       is set to true, and then it behaves as TimerEvo, with wait set to false once timer = \<delta>. \<close>
+
 definition 
   "EvolveUntil \<delta> a \<sigma> \<equiv> 
     T(timer ::= 0 ; wait ::= True ; TimerEvo \<delta> a \<sigma> (True)\<^sup>e ; 
       (IF timer \<ge> \<guillemotleft>\<delta>\<guillemotright> THEN wait ::= False ELSE skip)
      )"
 
-thm nmods_Choice
+text \<open> We now prove several useful results about EvolveUntil \<close>
 
 lemma
   assumes "vwb_lens a" "$t \<sharp> e" "$timer \<sharp> e" "$a \<sharp> e" "$wait \<sharp> e" 
   shows "EvolveUntil \<delta> a \<sigma> nmods e"
   using assms
-  apply (simp add: EvolveUntil_def TimerEvo_def)
+  apply (simp add: EvolveUntil_def TimerEvo_def T_def)
   apply (auto intro!: closure)
      apply (expr_auto)+
   done
-
-term "[a \<leadsto> b]"
-thm "unrest_expr"
-find_theorems "g_orbital_on"
-term "a\<lbrakk>v/x\<rbrakk>"
-term "( ($wait\<lbrakk>v/a\<rbrakk>)\<^sub>e = ($wait)\<^sub>e)"
-
-lemma "($wait\<lbrakk>1/timer\<rbrakk>)\<^sub>e = ($wait)\<^sub>e"
-  by (expr_auto)
-
-lemma "($wait\<lbrakk>wait/wait\<rbrakk>)\<^sub>e = ($wait)\<^sub>e"
-  by (expr_auto)
-
-lemma "($wait\<lbrakk>False/wait\<rbrakk>)\<^sub>e = (False)\<^sub>e"
-  by expr_auto
 
 lemma lens_indep_no_change:
   assumes "x \<bowtie> y" 
@@ -96,7 +121,8 @@ lemma lens_indep_no_change'[simp]:
   shows "get\<^bsub>x\<^esub> ([y \<leadsto> b] d) = get\<^bsub>x\<^esub> d"
   by (simp add: assms get_subst_upd_indep subst_id_def lens_indep_sym)
 
-(* This is a notion weaker than lens independence, but not sure if it's worth working with it! *)
+(* The above is a notion weaker than lens independence, as can be seen from the unfinished proof, 
+   but I'm not sure if it's worth working with it! *)
 lemma 
   assumes "(\<And>v. ($y\<lbrakk>v/x\<rbrakk>)\<^sub>e = ($y)\<^sub>e)"
   shows "x \<bowtie> y"
@@ -115,16 +141,20 @@ lemma
   apply expr_auto
   oops
 
-lemma EvolveUntil_not_wait:
-  (* Need assumption that a does not modify wait. Stated below using substitution:
-     essentially, it must be the case that for every possible state v, when
-     a is substituted in $wait by v, then its value doesn't change. *)
+text \<open> The following lemma confirms our intuition that provided EvolveUntil is started from a
+       state in which wait is not true, then when it terminates (\<not> wait) then timer = \<delta>. For
+       this result to hold we need to know that the lens a is independent from wait, so that
+       it does not modify it.
 
-  (* I've removed the assumption: (\<And>v. ($wait\<lbrakk>v/a\<rbrakk>)\<^sub>e = ($wait)\<^sub>e) in favour of lens independence,
+       In general this should always be the case, as ODEs should not be talking about wait.
+       Perhaps there could be a way to restrict the frame type? \<close>
+
+lemma EvolveUntil_not_wait:
+   (* I've removed the assumption: (\<And>v. ($wait\<lbrakk>v/a\<rbrakk>)\<^sub>e = ($wait)\<^sub>e) in favour of lens independence,
      which is stronger, but practically I think nearly always wanted for this result. *)
   assumes "a \<bowtie> wait"
   shows "\<^bold>{ \<not> wait \<^bold>} EvolveUntil \<delta> a \<sigma> \<^bold>{ \<not> wait \<longrightarrow> timer = \<guillemotleft>\<delta>\<guillemotright> \<^bold>}"
-  unfolding EvolveUntil_def
+  unfolding EvolveUntil_def T_def
   apply (rule hoare_if_then_else)
   apply ((simp only:kcomp_assoc)?, rule hoare_floyd_kcomp, simp)
    apply ((simp only:kcomp_assoc)?, rule hoare_floyd_kcomp, simp, subst_eval)
@@ -133,19 +163,11 @@ lemma EvolveUntil_not_wait:
     apply (rule TimerEvo_delta_nmods)
   unfolding TimerEvo_def apply (auto intro!:closure; subst_eval)
   using assms apply simp
-     (* (\<And>v. ?a\<lbrakk>v/?x\<rbrakk> = (?a)\<^sub>e) *)
     apply wlp_full+
   done
 
 (* Need a lemma that states: if the rate of change of a variable is
    the same as another, then they are changed by the same amount.*) 
-
-lemma hoare_T_wait:
-  assumes "\<^bold>{P \<and> \<not> wait\<^bold>} C \<^bold>{Q\<^bold>}" "`(P \<and> wait) \<longrightarrow> Q`"
-  shows "\<^bold>{P\<^bold>} T C \<^bold>{Q\<^bold>}"
-  apply (rule hoare_if_then_else)
-  using assms apply simp
-  by (metis (mono_tags, lifting) SEXP_def assms(2) fbox_skip predicate1I taut_def)
 
 lemma "vwb_lens a \<Longrightarrow> a \<bowtie> t \<Longrightarrow> a \<bowtie> timer \<Longrightarrow> vwb_lens (timer +\<^sub>L t +\<^sub>L a)"
   by (meson indeps(11) lens_indep_sym plus_pres_lens_indep' plus_vwb_lens vwbs(3) vwbs(4))
@@ -176,7 +198,7 @@ lemma plus_vwb_lens' [simp]:
 lemma TimerEvo_t_increasing:
   assumes "vwb_lens a" "t \<bowtie> a" "timer \<bowtie> a"
   shows "\<^bold>{ \<guillemotleft>t\<^sub>1\<guillemotright> \<le> t \<^bold>} TimerEvo \<delta> a \<sigma> (True)\<^sup>e \<^bold>{ \<guillemotleft>t\<^sub>1\<guillemotright> \<le> t \<^bold>}"
-  unfolding TimerEvo_def (* despite the above dInduct can fail if t \<bowtie> a is swapped by a \<bowtie> t *)
+  unfolding TimerEvo_def T_def (* despite the above dInduct can fail if t \<bowtie> a is swapped by a \<bowtie> t *)
   using assms by (dInduct)
  
 lemma TimerEvo_t_increasing':
@@ -190,6 +212,98 @@ lemma TimerEvo_timer_sum_invariant:
   shows " \<^bold>{ t = \<guillemotleft>t\<^sub>0\<guillemotright> + timer \<^bold>} TimerEvo \<delta> a \<sigma> (True)\<^sup>e \<^bold>{ t = \<guillemotleft>t\<^sub>0\<guillemotright> + timer \<^bold>}"
   using assms unfolding TimerEvo_def 
   by (dInduct)
+
+lemma T_increasing_t:
+  assumes "\<^bold>{ \<guillemotleft>t\<^sub>1\<guillemotright> \<le> t \<^bold>} X \<^bold>{ \<guillemotleft>t\<^sub>1\<guillemotright> \<le> t \<^bold>}"
+  shows "\<^bold>{ \<guillemotleft>t\<^sub>1\<guillemotright> \<le> t \<^bold>} T(X) \<^bold>{ \<guillemotleft>t\<^sub>1\<guillemotright> \<le> t \<^bold>}"
+  unfolding T_def 
+  apply (rule hoare_if_then_else)
+  using assms by wlp_full+  
+
+lemma T_kcomp_increasing_t:
+  assumes "\<^bold>{ \<guillemotleft>t\<^sub>1\<guillemotright> = t \<^bold>} X \<^bold>{ \<guillemotleft>t\<^sub>1\<guillemotright> \<le> t \<^bold>}" "\<^bold>{ \<guillemotleft>t\<^sub>1\<guillemotright> \<le> t \<^bold>} Y \<^bold>{ \<guillemotleft>t\<^sub>1\<guillemotright> \<le> t \<^bold>}" 
+  shows "\<^bold>{ \<guillemotleft>t\<^sub>1\<guillemotright> = t \<^bold>} T(X ; Y) \<^bold>{ \<guillemotleft>t\<^sub>1\<guillemotright> \<le> t \<^bold>}"
+  unfolding T_def 
+  apply (rule hoare_if_then_else)
+   defer
+   apply (smt (verit, best) SEXP_def fbox_skip predicate1I)
+  apply (rule hoare_kcomp[where R="(\<guillemotleft>t\<^sub>1\<guillemotright> \<le> t)\<^sup>e"])
+  using assms by auto
+
+lemma T_kcomp_increasing_t':
+  assumes "\<^bold>{ \<guillemotleft>t\<^sub>1\<guillemotright> \<le> t \<^bold>} X \<^bold>{ \<guillemotleft>t\<^sub>1\<guillemotright> \<le> t \<^bold>}" "\<^bold>{ \<guillemotleft>t\<^sub>1\<guillemotright> \<le> t \<^bold>} Y \<^bold>{ \<guillemotleft>t\<^sub>1\<guillemotright> \<le> t \<^bold>}" 
+  shows "\<^bold>{ \<guillemotleft>t\<^sub>1\<guillemotright> \<le> t \<^bold>} T(X ; Y) \<^bold>{ \<guillemotleft>t\<^sub>1\<guillemotright> \<le> t \<^bold>}"
+  unfolding T_def 
+  apply (rule hoare_if_then_else)
+   defer
+   apply (smt (verit, best) SEXP_def fbox_skip predicate1I)
+  apply (rule hoare_kcomp[where R="(\<guillemotleft>t\<^sub>1\<guillemotright> \<le> t)\<^sup>e"])
+  using assms by auto
+  
+lemma EvolveUntil_increasing_t:
+  assumes "vwb_lens a" "t \<bowtie> a" "timer \<bowtie> a"
+  shows "\<^bold>{ \<guillemotleft>t\<^sub>1\<guillemotright> = t \<^bold>} EvolveUntil \<delta>\<^sub>c a \<sigma> \<^bold>{ \<guillemotleft>t\<^sub>1\<guillemotright> \<le> t \<^bold>}"
+  unfolding EvolveUntil_def
+  apply (rule T_kcomp_increasing_t)
+   apply (subst kcomp_assoc)
+   apply (rule hoare_kcomp[where R="(\<guillemotleft>t\<^sub>1\<guillemotright> \<le> t)\<^sup>e"], wlp_full)
+  apply (rule hoare_kcomp[where R="(\<guillemotleft>t\<^sub>1\<guillemotright> \<le> t)\<^sup>e"], wlp_full)
+  using assms apply (simp add: TimerEvo_t_increasing)
+  apply (rule hoare_if_then_else, wlp_full)
+  by (wlp_full)
+
+lemma EvolveUntil_increasing_t':
+  assumes "vwb_lens a" "t \<bowtie> a" "timer \<bowtie> a"
+  shows "\<^bold>{ \<guillemotleft>t\<^sub>1\<guillemotright> \<le> t \<^bold>} EvolveUntil \<delta>\<^sub>c a \<sigma> \<^bold>{ \<guillemotleft>t\<^sub>1\<guillemotright> \<le> t \<^bold>}"
+  unfolding EvolveUntil_def
+  apply (rule T_kcomp_increasing_t')
+   apply (subst kcomp_assoc)
+   apply (rule hoare_kcomp[where R="(\<guillemotleft>t\<^sub>1\<guillemotright> \<le> t)\<^sup>e"], wlp_full)
+  apply (rule hoare_kcomp[where R="(\<guillemotleft>t\<^sub>1\<guillemotright> \<le> t)\<^sup>e"], wlp_full)
+  using assms apply (simp add: TimerEvo_t_increasing)
+  apply (rule hoare_if_then_else, wlp_full)
+  by (wlp_full)
+
+
+lemma kstar_increasing_t:
+  assumes "\<^bold>{ \<guillemotleft>t\<^sub>1\<guillemotright> \<le> t \<^bold>} X \<^bold>{ \<guillemotleft>t\<^sub>1\<guillemotright> \<le> t \<^bold>}"
+  shows "\<^bold>{ \<guillemotleft>t\<^sub>1\<guillemotright> = t \<^bold>} X\<^sup>* \<^bold>{ \<guillemotleft>t\<^sub>1\<guillemotright> \<le> t \<^bold>}"
+  apply (subst kstar_zero_or_one_or_more)
+  apply (rule hoare_choice, wlp_full)
+  apply (rule hoare_kcomp[where R="(\<guillemotleft>t\<^sub>1\<guillemotright> \<le> t)\<^sup>e"])
+   apply (rule hoare_weaken_pre_conj[where P="(\<guillemotleft>t\<^sub>1\<guillemotright> \<le> t)\<^sup>e"], simp)
+  using assms apply simp
+  apply (rule hoare_kstar_inv)
+  using assms by auto
+
+lemma kstar_increasing_t':
+  assumes "\<^bold>{ \<guillemotleft>t\<^sub>1\<guillemotright> \<le> t \<^bold>} X \<^bold>{ \<guillemotleft>t\<^sub>1\<guillemotright> \<le> t \<^bold>}"
+  shows "\<^bold>{ \<guillemotleft>t\<^sub>1\<guillemotright> \<le> t \<^bold>} X\<^sup>* \<^bold>{ \<guillemotleft>t\<^sub>1\<guillemotright> \<le> t \<^bold>}"
+  apply (subst kstar_zero_or_one_or_more)
+  apply (rule hoare_choice, wlp_full)
+  apply (rule hoare_kcomp[where R="(\<guillemotleft>t\<^sub>1\<guillemotright> \<le> t)\<^sup>e"])
+   apply (rule hoare_weaken_pre_conj[where P="(\<guillemotleft>t\<^sub>1\<guillemotright> \<le> t)\<^sup>e"], simp)
+  using assms apply simp
+  apply (rule hoare_kstar_inv)
+  using assms by auto
+
+lemma T_EvolveUntil_kstar_increasting_t:
+  assumes "vwb_lens a" "t \<bowtie> a" "timer \<bowtie> a" "\<^bold>{\<guillemotleft>t\<^sub>0\<guillemotright> \<le> t\<^bold>} T C \<^bold>{\<guillemotleft>t\<^sub>0\<guillemotright> \<le> t\<^bold>}"
+  shows "\<^bold>{\<guillemotleft>t\<^sub>0\<guillemotright> = t\<^bold>} (T C ; EvolveUntil \<delta> a \<sigma>)\<^sup>* \<^bold>{\<guillemotleft>t\<^sub>0\<guillemotright> \<le> t\<^bold>}"
+  apply (rule kstar_increasing_t)
+  apply (rule hoare_kcomp[where R="(\<guillemotleft>t\<^sub>0\<guillemotright> \<le> t)\<^sup>e"])
+   defer
+  using assms(1-3) apply (rule EvolveUntil_increasing_t')
+  using assms(4) by auto
+
+lemma T_EvolveUntil_kstar_increasting_t':
+  assumes "vwb_lens a" "t \<bowtie> a" "timer \<bowtie> a" "\<^bold>{\<guillemotleft>t\<^sub>0\<guillemotright> \<le> t\<^bold>} T C \<^bold>{\<guillemotleft>t\<^sub>0\<guillemotright> \<le> t\<^bold>}"
+  shows "\<^bold>{\<guillemotleft>t\<^sub>0\<guillemotright> \<le> t\<^bold>} (T C ; EvolveUntil \<delta> a \<sigma>)\<^sup>* \<^bold>{\<guillemotleft>t\<^sub>0\<guillemotright> \<le> t\<^bold>}"
+  apply (rule kstar_increasing_t')
+  apply (rule hoare_kcomp[where R="(\<guillemotleft>t\<^sub>0\<guillemotright> \<le> t)\<^sup>e"])
+   defer
+  using assms(1-3) apply (rule EvolveUntil_increasing_t')
+  using assms(4) by auto
 
 lemma TimerEvo_timer_sum_invariant':
   assumes "vwb_lens a" "t \<bowtie> a" "timer \<bowtie> a"
@@ -236,9 +350,9 @@ lemma EvolveUntil_t_not_wait:
   (* Need assumption that a does not modify wait. Stated below using substitution:
      essentially, it must be the case that for every possible state v, when
      a is substituted in $wait by v, then its value doesn't change. *)
-  assumes "a \<bowtie> wait" "TimerEvo \<delta> a \<sigma> (True)\<^sup>e nmods P" "$wait \<sharp> P" "$timer \<sharp> P" "vwb_lens a" "t \<bowtie> a" "timer \<bowtie> a"
+  assumes "a \<bowtie> wait" "\<^bold>{P\<^bold>} TimerEvo \<delta> a \<sigma> (True)\<^sup>e \<^bold>{P\<^bold>}" "$wait \<sharp> P" "$timer \<sharp> P" "vwb_lens a" "t \<bowtie> a" "timer \<bowtie> a"
   shows "\<^bold>{ P \<and> t = \<guillemotleft>t\<^sub>0\<guillemotright> \<and> \<not> wait \<^bold>} EvolveUntil \<delta> a \<sigma> \<^bold>{ P \<and> (\<not> wait \<longleftrightarrow> t = \<guillemotleft>t\<^sub>0\<guillemotright> + \<guillemotleft>\<delta>\<guillemotright>) \<and> (wait \<longleftrightarrow> t < \<guillemotleft>t\<^sub>0\<guillemotright> + \<guillemotleft>\<delta>\<guillemotright>)\<^bold>}"
-  unfolding EvolveUntil_def
+  unfolding EvolveUntil_def T_def
    apply (rule hoare_if_then_else)
     apply ((simp only:kcomp_assoc)?, rule hoare_floyd_kcomp, simp)
    apply ((simp only:kcomp_assoc)?, rule hoare_floyd_kcomp, simp, subst_eval)
@@ -254,14 +368,16 @@ lemma EvolveUntil_t_not_wait:
   apply (rule hoare_conj_posI[where a="(P \<and> wait \<and> t = \<guillemotleft>t\<^sub>0\<guillemotright> + timer)\<^sup>e" and b="(timer \<le> \<guillemotleft>\<delta>\<guillemotright>)\<^sup>e"])
     defer
     apply (simp add: TimerEvo_pos_timer_delta)
-  apply expr_auto
-  apply (rule nmods_frame_law'', simp add:assms)
+   apply expr_auto
+  apply (rule hoare_conj_inv)
+  apply (simp add:assms) 
   apply (rule nmods_frame_law'', simp add:assms TimerEvo_nmods_lens)
-  by (simp add:assms TimerEvo_timer_sum_invariant) 
+  by (simp add:assms TimerEvo_timer_sum_invariant)
 
+(*
 lemma 
   assumes "a \<bowtie> wait" 
-          "TimerEvo \<delta> a \<sigma> (True)\<^sup>e nmods P" (* Might want to relax this assumption. *)
+          "\<^bold>{P\<^bold>} TimerEvo \<delta> a \<sigma> (True)\<^sup>e \<^bold>{P\<^bold>}" (* Might want to relax this assumption. *)
           "$wait \<sharp> P" "$timer \<sharp> P" "vwb_lens a" "t \<bowtie> a" "timer \<bowtie> a"
           "`(P \<and> t = \<guillemotleft>t\<^sub>0\<guillemotright> + \<guillemotleft>\<delta>\<guillemotright>) \<longrightarrow> R`"
          (* "\<^bold>{ t = \<guillemotleft>t\<^sub>1\<guillemotright> \<^bold>} C \<^bold>{ \<guillemotleft>t\<^sub>1\<guillemotright> \<le> t \<^bold>}" *)
@@ -273,7 +389,7 @@ lemma
            * it holds at t = t\<^sub>0 + \<delta> as established by EvolveUntil at t = t\<^sub>0 + \<delta>,
              so perhaps it is sufficient to show that `P \<and> t = t\<^sub>0 + \<delta> \<longrightarrow> R` ?
     *)
-  shows "\<^bold>{P \<and> t = \<guillemotleft>t\<^sub>0\<guillemotright> \<and> \<not> wait\<^bold>} EvolveUntil \<delta> a \<sigma> ; T(C) \<^bold>{t \<le> \<guillemotleft>t\<^sub>0\<guillemotright> + \<guillemotleft>\<delta>\<guillemotright> \<longrightarrow> P \<and> \<guillemotleft>t\<^sub>0\<guillemotright> + \<guillemotleft>\<delta>\<guillemotright> \<le> t \<longrightarrow> R\<^bold>}"
+  shows "\<^bold>{P \<and> t = \<guillemotleft>t\<^sub>0\<guillemotright> \<and> \<not> wait\<^bold>} EvolveUntil \<delta> a \<sigma> ; T(C) \<^bold>{(t \<le> \<guillemotleft>t\<^sub>0\<guillemotright> + \<guillemotleft>\<delta>\<guillemotright> \<longrightarrow> P) \<and> (\<guillemotleft>t\<^sub>0\<guillemotright> + \<guillemotleft>\<delta>\<guillemotright> \<le> t \<longrightarrow> R)\<^bold>}"
   apply (rule hoare_kcomp[where R="(P \<and> (\<not> wait \<longleftrightarrow> t = \<guillemotleft>t\<^sub>0\<guillemotright> + \<guillemotleft>\<delta>\<guillemotright>) \<and> (wait \<longleftrightarrow> t < \<guillemotleft>t\<^sub>0\<guillemotright> + \<guillemotleft>\<delta>\<guillemotright>))\<^sup>e"])
   using assms apply (simp only:EvolveUntil_t_not_wait) (* Tentative *)
   apply (rule hoare_T_wait) (* Need C to be monotonically increasing on t *)
@@ -281,11 +397,147 @@ lemma
   apply expr_auto
   apply (rule hoare_weaken_pre_conj[where P="(P \<and> \<not> wait \<and> t = \<guillemotleft>t\<^sub>0\<guillemotright> + \<guillemotleft>\<delta>\<guillemotright> \<and> R)\<^sup>e"])
   using assms apply expr_auto
-  apply (rule hoare_weaken_pre_conj[where P="(R)\<^sup>e"], expr_auto)
+  apply (rule hoare_weaken_pre_conj[where P="(R \<and> t = \<guillemotleft>t\<^sub>0\<guillemotright> + \<guillemotleft>\<delta>\<guillemotright>)\<^sup>e"], expr_auto)
   apply (rule hoare_stengthen_post[where Q="(R)\<^sup>e"])
-  using assms apply expr_auto
+  using assms apply simp
+  using assms by auto *)
+
+lemma 
+  assumes "vwb_lens a" "t \<bowtie> a" "timer \<bowtie> a" "\<^bold>{$a = a\<^sub>0\<^bold>} TimerEvo \<delta>\<^sub>s a \<sigma> (True)\<^sup>e \<^bold>{$a = a\<^sub>0\<^bold>}"
+  shows "TimerEvo \<delta>\<^sub>s a \<sigma> (True)\<^sup>e = {timer` = 1, t` = 1 | timer \<le> \<delta>}"
+  using assms unfolding TimerEvo_def oops
+
+lemma T_kcomp_fixpoint:
+  shows "T(T(P) ; T(Q)) = T(P) ; T(Q)"
+  unfolding T_def ifthenelse_def skip_def kcomp_def by expr_auto
+
+lemma T_kstar_fixpoint:
+  shows "T((T(P))\<^sup>*) = (T(P))\<^sup>*"
+  unfolding T_def ifthenelse_def skip_def kstar_def apply expr_auto
+   apply (metis (full_types) kpower_0 singletonI)
+  by (smt (verit, ccfv_SIG) Collect_conv_if2 kpower_inv mem_Collect_eq)
+
+lemma T_EvolveUntil_fixpoint:
+  shows "(T C ; EvolveUntil \<delta>\<^sub>c a \<sigma>)\<^sup>* = T((T C ; EvolveUntil \<delta>\<^sub>c a \<sigma>)\<^sup>*)"
+  using T_kstar_fixpoint 
+  by (smt (verit, ccfv_threshold) EvolveUntil_def T_kcomp_fixpoint)
+
+lemma T_EvolveUntil_plus_fixpoint:
+  shows "(T C ; EvolveUntil \<delta>\<^sub>c a \<sigma>)\<^sup>+ = T((T C ; EvolveUntil \<delta>\<^sub>c a \<sigma>)\<^sup>+)"
+  using T_kstar_fixpoint unfolding kstar_one_def
+  by (smt (verit, ccfv_threshold) EvolveUntil_def T_kcomp_fixpoint)
+
+lemma T_invariant:
+  assumes "\<^bold>{R\<^bold>} C \<^bold>{R\<^bold>}"
+  shows "\<^bold>{R\<^bold>} T C \<^bold>{R\<^bold>}"
+  unfolding T_def 
+  apply (rule hoare_if_then_else')
+  using assms apply simp
+  by (simp add: hoare_skip)
+
+lemma hoare_pre_eq:
+  assumes "\<^bold>{Q\<^bold>} X \<^bold>{S\<^bold>}" "R = Q"
+  shows "\<^bold>{R\<^bold>} X \<^bold>{S\<^bold>}"
   using assms by auto
-  
+
+lemma EvolveUntil_two_post:
+  assumes "a \<bowtie> wait" 
+          "\<^bold>{P\<^bold>} TimerEvo \<delta> a \<sigma> (True)\<^sup>e \<^bold>{P\<^bold>}" (* Might want to relax this assumption. *)
+          "$wait \<sharp> P" "$timer \<sharp> P" "vwb_lens a" "t \<bowtie> a" "timer \<bowtie> a"
+          (* "\<^bold>{P \<and> t = \<guillemotleft>t\<^sub>0\<guillemotright> + \<guillemotleft>\<delta>\<guillemotright>\<^bold>} C \<^bold>{R\<^bold>}"*) "`(P \<and> t = \<guillemotleft>t\<^sub>0\<guillemotright> + \<guillemotleft>\<delta>\<guillemotright>) \<longrightarrow> R`" (* This may a little too strong *)
+          "\<And>t\<^sub>1. \<^bold>{ \<guillemotleft>t\<^sub>1\<guillemotright> \<le> t \<^bold>} C \<^bold>{ \<guillemotleft>t\<^sub>1\<guillemotright> \<le> t \<^bold>}"
+          "\<^bold>{R\<^bold>} C \<^bold>{R\<^bold>}"
+          "\<^bold>{R\<^bold>} EvolveUntil \<delta>\<^sub>c a \<sigma> \<^bold>{R\<^bold>}"
+  shows "\<^bold>{P \<and> t = \<guillemotleft>t\<^sub>0\<guillemotright> \<and> \<not> wait\<^bold>}
+         EvolveUntil \<delta> a \<sigma> ; (T(C) ; EvolveUntil \<delta>\<^sub>c a \<sigma>)\<^sup>*
+         \<^bold>{(t < \<guillemotleft>t\<^sub>0\<guillemotright> + \<guillemotleft>\<delta>\<guillemotright> \<longrightarrow> P) \<and> (\<guillemotleft>t\<^sub>0\<guillemotright> + \<guillemotleft>\<delta>\<guillemotright> \<le> t \<longrightarrow> R)\<^bold>}"
+  apply (rule hoare_kcomp[where R="(P \<and> (\<not> wait \<longleftrightarrow> t = \<guillemotleft>t\<^sub>0\<guillemotright> + \<guillemotleft>\<delta>\<guillemotright>) \<and> (wait \<longleftrightarrow> t < \<guillemotleft>t\<^sub>0\<guillemotright> + \<guillemotleft>\<delta>\<guillemotright>))\<^sup>e"])
+  using assms apply (simp only:EvolveUntil_t_not_wait) (* Tentative *)
+  apply (subst T_EvolveUntil_fixpoint)
+  apply (rule hoare_T_wait) (* Need C to be monotonically increasing on t *)
+   defer
+  apply expr_auto
+  apply (rule hoare_weaken_pre_conj[where P="(P \<and> \<not> wait \<and> t = \<guillemotleft>t\<^sub>0\<guillemotright> + \<guillemotleft>\<delta>\<guillemotright>)\<^sup>e"])
+  using assms apply expr_auto
+(* Use: T_EvolveUntil_kstar_increasting_t *)
+  using assms apply (insert T_increasing_t[where t\<^sub>1="t\<^sub>0 + \<delta>" and X="C"])
+  apply (insert T_EvolveUntil_kstar_increasting_t[where C="C" and t\<^sub>0="t\<^sub>0 + \<delta>" and \<delta>="\<delta>\<^sub>c" and a="a" and \<sigma>="\<sigma>"])
+  using assms apply simp
+  apply (rule hoare_stengthen_post[where Q="(\<guillemotleft>t\<^sub>0\<guillemotright> + \<guillemotleft>\<delta>\<guillemotright> \<le> t \<and> R)\<^sup>e"], expr_simp)
+  thm hoare_conj_posI
+  apply (rule hoare_conj_posI[where a="(\<guillemotleft>t\<^sub>0\<guillemotright> + \<guillemotleft>\<delta>\<guillemotright> \<le> t)\<^sup>e" and b="R"])
+    defer
+    defer
+  apply expr_simp
+  apply (rule hoare_weaken_pre_conj[where P="(t = \<guillemotleft>t\<^sub>0\<guillemotright> + \<guillemotleft>\<delta>\<guillemotright>)\<^sup>e"], expr_auto)
+    apply (smt (verit, best) SEXP_def le_fun_def)
+      apply (rule hoare_weaken_pre_conj[where P="(R \<and> \<not> wait \<and> t = \<guillemotleft>t\<^sub>0\<guillemotright> + \<guillemotleft>\<delta>\<guillemotright>)\<^sup>e"], expr_auto)
+(*  apply (rule hoare_stengthen_post[where Q="(R)\<^sup>e"])
+  using assms apply simp*)
+  apply (subst kstar_zero_or_one_or_more)
+  apply (rule hoare_choice)
+   apply (simp add:fbox_skip, expr_auto)
+  apply (subst kcomp_assoc)
+  apply (rule hoare_kcomp[where R="(R)\<^sup>e"])
+   apply (rule hoare_T_wait, simp)
+    apply (rule hoare_weaken_pre_conj[where P="(R)\<^sup>e"], expr_auto)
+  using assms apply simp
+   apply expr_auto
+  apply (rule hoare_kcomp[where R="(R)\<^sup>e"])
+  using assms apply simp
+  apply (rule hoare_kstar_inv)
+  apply (rule hoare_kcomp[where R="(R)\<^sup>e"])
+  using assms by (auto simp add:T_invariant)
+
+lemma EvolveUntil_two_post_plus:
+  assumes "a \<bowtie> wait" 
+          "\<^bold>{P\<^bold>} TimerEvo \<delta> a \<sigma> (True)\<^sup>e \<^bold>{P\<^bold>}" (* Might want to relax this assumption. *)
+          "$wait \<sharp> P" "$timer \<sharp> P" "vwb_lens a" "t \<bowtie> a" "timer \<bowtie> a"
+          "\<^bold>{P \<and> t = \<guillemotleft>t\<^sub>0\<guillemotright> + \<guillemotleft>\<delta>\<guillemotright>\<^bold>} C \<^bold>{R \<and> t = \<guillemotleft>t\<^sub>0\<guillemotright> + \<guillemotleft>\<delta>\<guillemotright>\<^bold>}" (*"`(P \<and> t = \<guillemotleft>t\<^sub>0\<guillemotright> + \<guillemotleft>\<delta>\<guillemotright>) \<longrightarrow> R`"*) (* This may a little too strong *)
+          "\<And>t\<^sub>1. \<^bold>{ \<guillemotleft>t\<^sub>1\<guillemotright> \<le> t \<^bold>} C \<^bold>{ \<guillemotleft>t\<^sub>1\<guillemotright> \<le> t \<^bold>}"
+          "\<^bold>{R\<^bold>} C \<^bold>{R\<^bold>}"
+          "\<^bold>{R\<^bold>} EvolveUntil \<delta>\<^sub>c a \<sigma> \<^bold>{R\<^bold>}"
+  shows "\<^bold>{P \<and> t = \<guillemotleft>t\<^sub>0\<guillemotright> \<and> \<not> wait\<^bold>}
+         EvolveUntil \<delta> a \<sigma> ; (T(C) ; EvolveUntil \<delta>\<^sub>c a \<sigma>)\<^sup>+
+         \<^bold>{(t < \<guillemotleft>t\<^sub>0\<guillemotright> + \<guillemotleft>\<delta>\<guillemotright> \<longrightarrow> P) \<and> (\<guillemotleft>t\<^sub>0\<guillemotright> + \<guillemotleft>\<delta>\<guillemotright> \<le> t \<longrightarrow> R)\<^bold>}"
+  apply (rule hoare_kcomp[where R="(P \<and> (\<not> wait \<longleftrightarrow> t = \<guillemotleft>t\<^sub>0\<guillemotright> + \<guillemotleft>\<delta>\<guillemotright>) \<and> (wait \<longleftrightarrow> t < \<guillemotleft>t\<^sub>0\<guillemotright> + \<guillemotleft>\<delta>\<guillemotright>))\<^sup>e"])
+  using assms apply (simp only:EvolveUntil_t_not_wait) (* Tentative *)
+  apply (subst T_EvolveUntil_plus_fixpoint)
+  apply (rule hoare_T_wait) (* Need C to be monotonically increasing on t *)
+   defer
+  apply expr_auto
+  apply (rule hoare_weaken_pre_conj[where P="((P \<and> t = \<guillemotleft>t\<^sub>0\<guillemotright> + \<guillemotleft>\<delta>\<guillemotright>) \<and> \<not> wait )\<^sup>e"])
+  using assms apply expr_auto
+  unfolding kstar_one_def
+  apply (rule hoare_kcomp[where R="(\<guillemotleft>t\<^sub>0\<guillemotright> + \<guillemotleft>\<delta>\<guillemotright> \<le> t \<and> R)\<^sup>e"])
+  defer
+(* Proof steps unchanged below *)
+(* Use: T_EvolveUntil_kstar_increasting_t *)
+  using assms apply (insert T_increasing_t[where t\<^sub>1="t\<^sub>0 + \<delta>" and X="C"])
+  apply (insert T_EvolveUntil_kstar_increasting_t'[where C="C" and t\<^sub>0="t\<^sub>0 + \<delta>" and \<delta>="\<delta>\<^sub>c" and a="a" and \<sigma>="\<sigma>"])
+  using assms apply simp
+  apply (rule hoare_stengthen_post[where Q="(\<guillemotleft>t\<^sub>0\<guillemotright> + \<guillemotleft>\<delta>\<guillemotright> \<le> t \<and> R)\<^sup>e"], expr_simp)
+  thm hoare_conj_posI
+   apply (rule hoare_conj_posI[where a="(\<guillemotleft>t\<^sub>0\<guillemotright> + \<guillemotleft>\<delta>\<guillemotright> \<le> t)\<^sup>e" and b="R"])
+     apply (rule hoare_weaken_pre_conj[where P="(\<guillemotleft>t\<^sub>0\<guillemotright> + \<guillemotleft>\<delta>\<guillemotright> \<le> t)\<^sup>e"], expr_auto, simp)
+    defer
+    apply expr_simp
+  defer
+   apply (rule hoare_weaken_pre_conj[where P="(R)\<^sup>e"], simp)
+   apply (meson hoare_kcomp hoare_kstar_inv robosim.T_invariant robosim_axioms)
+  apply (rule hoare_kcomp[where R="(\<guillemotleft>t\<^sub>0\<guillemotright> + \<guillemotleft>\<delta>\<guillemotright> \<le> t \<and> R)\<^sup>e"])
+   apply (rule hoare_T_wait')
+   defer
+   apply (rule hoare_conj_inv)
+  using EvolveUntil_increasing_t' assms(5) assms(6) assms(7) apply blast
+  using assms apply blast
+  apply (rule hoare_stengthen_post[where Q="(R \<and> t = \<guillemotleft>t\<^sub>0\<guillemotright> + \<guillemotleft>\<delta>\<guillemotright>)\<^sup>e"], expr_simp)
+  using assms by auto
+  (*apply (rule hoare_conj_pos')
+  apply (rule hoare_weaken_pre_conj[where P="(\<guillemotleft>t\<^sub>0\<guillemotright> + \<guillemotleft>\<delta>\<guillemotright> \<le> t)\<^sup>e"], simp)
+  using assms(9) apply fastforce
+  using assms by auto*)
+
 lemma ini_cycle_loop:
   assumes "\<^bold>{P\<^bold>} I \<^bold>{P\<^bold>}" "\<^bold>{P\<^bold>} C \<^bold>{Q\<^bold>}" "\<^bold>{Q\<^bold>} C \<^bold>{Q\<^bold>}" "\<^bold>{Q\<^bold>} E \<^bold>{Q\<^bold>}"
   shows "\<^bold>{P\<^bold>} I ; C ; ((IF \<guillemotleft>TimeScale\<guillemotright>*\<guillemotleft>Cycle\<guillemotright> \<le> timer THEN C ELSE skip) ; E)\<^sup>* \<^bold>{Q\<^bold>}"
@@ -359,6 +611,39 @@ lemma cycle_loop'':
   shows "\<^bold>{P\<^bold>} (C ; E)\<^sup>* \<^bold>{R\<^bold>}"
   oops (* TBC *)
 
+lemma exists_subst [usubst_eval]:
+  "(Q \<and> R \<and> S \<and> (\<exists>v. v \<and> P))\<^sub>e = (Q \<and> R \<and> S \<and> P)\<^sub>e"
+  by wlp_full
+
+lemma exists_subst' [usubst_eval]:
+  "(Q \<and> (\<exists>v. v \<and> P))\<^sub>e = (Q \<and> P)\<^sub>e"
+  by wlp_full
+
+lemma exists_true [usubst_eval]:
+  "(\<exists>v. v)"
+  by wlp_full
+
+lemma exists_move [usubst_eval]:
+  "(Q \<and> (\<exists>v. v \<and> P))\<^sub>e = (Q \<and> (\<exists>v. P))\<^sub>e"
+  by wlp_full
+
+lemma EvolveUntil_TimerEvo:
+  assumes "$timer \<sharp> I" "$wait \<sharp> I" "\<^bold>{ I \<^bold>} TimerEvo \<delta> a \<sigma> (\<lambda>\<s>. True) \<^bold>{ I \<^bold>}"
+  shows "\<^bold>{ I \<^bold>} EvolveUntil \<delta> a \<sigma> \<^bold>{ I \<^bold>}"
+  unfolding EvolveUntil_def T_def
+  apply (rule hoare_if_then_else)
+   defer
+   apply wlp_full
+  thm nmods_invariant
+  apply ((simp only:kcomp_assoc)?, rule hoare_floyd_kcomp, simp, simp add:unrest usubst assms)
+  apply ((simp only:kcomp_assoc)?, rule hoare_floyd_kcomp, simp, simp add:unrest usubst assms)
+  apply (rule hoare_weaken_pre_conj[where P="I"], simp)
+  apply (rule hoare_kcomp[where R="I"])
+  using assms apply simp
+  apply (rule hoare_if_then_else)
+  using assms apply wlp_full
+  by wlp_full
+  
 end
 
 term "[\<leadsto>] \<circ>\<^sub>s \<sigma>(x \<leadsto> u, x \<leadsto> v)"
@@ -375,5 +660,24 @@ begin
 (* abbreviation (input) "TimerEvo \<delta> a \<sigma> B \<equiv> g_dl_ode_frame a \<sigma> (@B \<and> $timer \<le> \<delta>)\<^sub>e" *)
 
 end
+
+method hoare_help uses add = ( 
+    (
+      (simp only:kcomp_assoc)?, 
+      (   (rule hoare_else_kcomp, force) 
+        | (rule hoare_floyd_kcomp, simp, simp add: usubst_eval usubst unrest)
+        | (rule hoare_if_kcomp, force) 
+        | (rule hoare_ifte_kcomp)
+        | (rule hoare_pre_not_while_seq, simp, hoare_wp_auto)
+        | (rule hoare_pre_not_while, simp, hoare_wp_auto)
+        | (simp only:kcomp_skip)
+        | (dInduct_mega)
+        | (rule nmods_invariant, (clarify intro!:closure, subst_eval))
+        | (rule hoare_false, subst_eval)
+        | (simp add:unrest usubst expr_simps add)
+       )
+     )+, 
+   (subst WHILE_unroll_IF[symmetric])?
+  )+
 
 end
